Replaced efficient orset

code/mrdts/OR-set-efficient/App_mrdt.fst
@@ -3,39 +3,34 @@ module App_mrdt
 module S = Set_extended
 module M = Map_extended
 
-let enable_wins_flag = (int * bool)
+type replica_id : eqtype = nat
+type element : eqtype = nat
+type timestamp : eqtype = pos
 
 // the concrete state type
-type concrete_st = M.t nat (M.t nat enable_wins_flag)
-  // element -> replica ID -> enable-wins flag
+type concrete_st = S.t (replica_id & timestamp & element)
+  // Behaves as a [replica_id -> element -> timestamp]. That is, for each
+  // [replica_id], every [element] occurs uniquely.
+  //
   // Uses [O(n * r)] space where
   //    n = number of elements in the set
   //    r = number of replicas
-  // Has Tombstones
 
 // init state
-let init_st : concrete_st = M.const (M.const (0, false))
-
-let sel_id (s:M.t nat enable_wins_flag) id = if M.contains s id then M.sel s id else (0, false)
-
-let sel (s:concrete_st) e = if M.contains s e then M.sel s e else (M.const (0, false))
-
-// equivalence relation of ew flag
-let eq_e (a b:M.t nat enable_wins_flag) =
-  (forall id. M.contains a id = M.contains b id /\ sel_id a id = sel_id b id)
+let init_st : concrete_st = S.empty
 
 // equivalence between 2 concrete states
-let eq (a b:concrete_st) =
- (forall e. M.contains a e = M.contains b e /\ eq_e (sel a e) (sel b e))
+let eq (a b:concrete_st) : Type0 =
+  a == b
 
 let symmetric a b = ()
 
-let transitive a b enable_wins_flag = ()
+let transitive a b c = ()
 
 let eq_is_equiv a b = ()
 
 // operation type
-type app_op_t:eqtype =
+type app_op_t : eqtype =
   |Add : nat -> app_op_t
   |Rem : nat -> app_op_t
 
@@ -46,9 +41,23 @@ let get_ele (o:op_t) : nat =
 
 // apply an operation to a state
 let do (s:concrete_st) (o:op_t) : concrete_st =
- match o with
-  |(_, (rid, Add e)) -> M.upd s e (M.upd (sel s e) rid (fst (sel_id (sel s e) rid) + 1, true))
-  |(_, (rid, Rem e)) -> M.iter_upd (fun k v -> if k = e then ((M.map_val (fun (enable_wins_flag,f) -> (enable_wins_flag, false))) v) else v) s
+  match o with
+  | (ts, (rid, Add e)) ->
+    let s' = S.filter s (fun (rid',_,e') -> not (rid = rid' && e = e')) in
+    S.add (rid,ts,e) s'
+  | (_, (rid, Rem e)) ->
+    S.filter s (fun (_,_,e') -> not (e = e'))
+
+let test () =
+  let s1 = do init_st (1, (1, Add 0)) in
+  let s1' = S.singleton (1,1,0) in
+  assert (eq s1 s1');
+  let s2 = do s1 (2, (1, Add 0)) in
+  let s2' = S.singleton (1,2,0) in
+  assert (eq s2 s2');
+  let s3 = do s2 (3, (2, Add 0)) in
+  let s3' = S.add (2,3,0) s2' in
+  assert (eq s3 s3')
 
 //conflict resolution
 let rc (o1 o2:op_t) =
@@ -57,38 +66,20 @@ let rc (o1 o2:op_t) =
   |Rem e1, Add e2 -> if e1 = e2 then Fst_then_snd else Either
   |_ -> Either
 
-let merge_flag (l a b:enable_wins_flag) : bool =
-  let lc = fst l in
-  let ac = fst a in
-  let bc = fst b in
-  let af = snd a in
-  let bf = snd b in
-    if af && bf then true
-      else if not af && not bf then false
-        else if af then ac > lc
-          else bc > lc
+let merge (l a b : concrete_st) : concrete_st =
+  let da = S.difference a l in    //a - l
+  let db = S.difference b l in    //b - l
+  let i_ab = S.intersection a b in
+  let i_lab = S.intersection l i_ab in   // intersect l a b
+  S.union i_lab (S.union da db)          // (intersect l a b) U (a - l) U (b - l)
 
-// concrete merge operation
-let merge_cf (l a b:enable_wins_flag) : enable_wins_flag =
-  (fst a + fst b - fst l, merge_flag l a b)
+  /////////////////////////////////////////////////////////////////////////////
 
-// concrete merge operation
-let merge_ew (l a b:(M.t nat enable_wins_flag)) : (M.t nat enable_wins_flag) =
-  let keys = S.union (M.domain l) (S.union (M.domain a) (M.domain b)) in
-  let u = M.const_on keys (0, false) in
-  M.iter_upd (fun k v -> merge_cf (sel_id l k) (sel_id a k) (sel_id b k)) u
-
-// concrete merge operation
-let merge (l a b:concrete_st) : concrete_st =
-  let eles = S.union (M.domain l) (S.union (M.domain a) (M.domain b)) in
-  let u = M.const_on eles init_st in
-  M.iter_upd (fun k v -> merge_ew (sel l k) (sel a k) (sel b k)) u
-
-/////////////////////////////////////////////////////////////////////////////
-
+#push-options "--z3rlimit 100 --max_ifuel 3"
 let rc_non_comm_help1 (o1 o2:op_t)
-  : Lemma (ensures (((Add? (snd (snd o1)) /\ Rem? (snd (snd o2))) \/ (Rem? (snd (snd o1)) /\ Add? (snd (snd o2)))) /\ get_ele o1 = get_ele o2)
-  ==> ~ (eq (do (do init_st o1) o2) (do (do init_st o2) o1))) = ()
+  : Lemma (requires distinct_ops o1 o2)
+          (ensures (((Add? (snd (snd o1)) /\ Rem? (snd (snd o2))) \/ (Rem? (snd (snd o1)) /\ Add? (snd (snd o2)))) /\ get_ele o1 = get_ele o2) ==>
+                           ~ (eq (do (do init_st o1) o2) (do (do init_st o2) o1))) = ()
 
 let rc_non_comm o1 o2 =
   rc_non_comm_help1 o1 o2
@@ -97,272 +88,50 @@ let no_rc_chain o1 o2 o3 = ()
 
 let cond_comm_base s o1 o2 o3 = ()
 
-#set-options "--z3rlimit 200 --ifuel 5"
 let cond_comm_ind s o1 o2 o3 o l = ()
 
-/////////////////////////////////////////////////////////////////////////////
-// Merge commutativity
-let merge_comm (l a b:concrete_st)
-   : Lemma (ensures (eq (merge l a b) (merge l b a))) = ()
+/////////////////////////////////// Verification Conditions //////////////////////////////////////////
 
-// Merge idempotence
-let merge_idem (s:concrete_st)
-   : Lemma (ensures eq (merge s s s) s) = ()
+let merge_comm l a b = ()
 
-///////////////////////////////////////////////////////////////////////////
+let merge_idem s = ()
 
 let base_2op o1 o2 = ()
 
-let ind_lca_2op_fts (l:concrete_st) (o1 o2 ol:op_t)
-  : Lemma (requires Rem? (snd (snd o2)) /\ Add? (snd (snd o1)) /\
-                    eq (merge l (do l o1) (do l o2)) (do (merge l l (do l o2)) o1))
-          (ensures eq (merge (do l ol) (do (do l ol) o1) (do (do l ol) o2)) (do (merge (do l ol) (do l ol) (do (do l ol) o2)) o1)) = ()
+let ind_lca_2op l o1 o2 ol = ()
 
-let ind_lca_2op_comm1 (l:concrete_st) (o1 o2 ol:op_t)
-  : Lemma (requires Add? (snd (snd o2)) /\ Add? (snd (snd o1)) /\
-                    eq (merge l (do l o1) (do l o2)) (do (merge l l (do l o2)) o1))
-          (ensures eq (merge (do l ol) (do (do l ol) o1) (do (do l ol) o2)) (do (merge (do l ol) (do l ol) (do (do l ol) o2)) o1)) = ()
-
-let ind_lca_2op_comm2 (l:concrete_st) (o1 o2 ol:op_t)
-  : Lemma (requires Rem? (snd (snd o2)) /\ Rem? (snd (snd o1)) /\
-                    eq (merge l (do l o1) (do l o2)) (do (merge l l (do l o2)) o1))
-          (ensures eq (merge (do l ol) (do (do l ol) o1) (do (do l ol) o2)) (do (merge (do l ol) (do l ol) (do (do l ol) o2)) o1)) = ()
-
-let ind_lca_2op_comm3 (l:concrete_st) (o1 o2 ol:op_t)
-  : Lemma (requires Add? (snd (snd o2)) /\ Rem? (snd (snd o1)) /\
-                    eq (merge l (do l o1) (do l o2)) (do (merge l l (do l o2)) o1))
-          (ensures eq (merge (do l ol) (do (do l ol) o1) (do (do l ol) o2)) (do (merge (do l ol) (do l ol) (do (do l ol) o2)) o1)) = ()
-
-let ind_lca_2op_comm4 (l:concrete_st) (o1 o2 ol:op_t)
-  : Lemma (requires Rem? (snd (snd o2)) /\ Add? (snd (snd o1)) /\
-                    eq (merge l (do l o1) (do l o2)) (do (merge l l (do l o2)) o1))
-          (ensures eq (merge (do l ol) (do (do l ol) o1) (do (do l ol) o2)) (do (merge (do l ol) (do l ol) (do (do l ol) o2)) o1)) = ()
-
-let ind_lca_2op l o1 o2 ol =
-  if Fst_then_snd? (rc o2 o1) then ind_lca_2op_fts l o1 o2 ol
-  else (if Add? (snd (snd o2)) && Add? (snd (snd o1)) then ind_lca_2op_comm1 l o1 o2 ol
-        else if Rem? (snd (snd o2)) && Rem? (snd (snd o1)) then ind_lca_2op_comm2 l o1 o2 ol
-        else if Add? (snd (snd o2)) && Rem? (snd (snd o1)) then ind_lca_2op_comm3 l o1 o2 ol
-        else ind_lca_2op_comm4 l o1 o2 ol)
-
-let inter_right_base_2op_fts (l a b :concrete_st) (o1 o2 ob ol:op_t)
-  : Lemma (requires Rem? (snd (snd o2)) /\ Add? (snd (snd o1)) /\
-                    Rem? (snd (snd ob)) /\ Add? (snd (snd ol)) /\
-                    eq (merge l (do a o1) (do (do b ob) o2)) (do (merge l a (do (do b ob) o2)) o1) /\ //from ind_right_2op
-                    eq (merge (do l ol) (do (do a ol) o1) (do (do b ol) o2)) (do (merge (do l ol) (do a ol) (do (do b ol) o2)) o1))
-          (ensures eq (merge (do l ol) (do (do a ol) o1) (do (do (do b ob) ol) o2)) (do (merge (do l ol) (do a ol) (do (do (do b ob) ol) o2)) o1)) = ()
-
-let inter_right_base_2op_comm1 (l a b :concrete_st) (o1 o2 ob ol:op_t)
-  : Lemma (requires Add? (snd (snd o2)) /\ Add? (snd (snd o1)) /\
-                    Rem? (snd (snd ob)) /\ Add? (snd (snd ol)) /\
-                    eq (merge l (do a o1) (do (do b ob) o2)) (do (merge l a (do (do b ob) o2)) o1) /\ //from ind_right_2op
-                    eq (merge (do l ol) (do (do a ol) o1) (do (do b ol) o2)) (do (merge (do l ol) (do a ol) (do (do b ol) o2)) o1))
-          (ensures eq (merge (do l ol) (do (do a ol) o1) (do (do (do b ob) ol) o2)) (do (merge (do l ol) (do a ol) (do (do (do b ob) ol) o2)) o1)) = ()
-
-let inter_right_base_2op_comm2 (l a b :concrete_st) (o1 o2 ob ol:op_t)
-  : Lemma (requires Rem? (snd (snd o2)) /\ Rem? (snd (snd o1)) /\
-                    Rem? (snd (snd ob)) /\ Add? (snd (snd ol)) /\
-                    eq (merge l (do a o1) (do (do b ob) o2)) (do (merge l a (do (do b ob) o2)) o1) /\ //from ind_right_2op
-                    eq (merge (do l ol) (do (do a ol) o1) (do (do b ol) o2)) (do (merge (do l ol) (do a ol) (do (do b ol) o2)) o1))
-          (ensures eq (merge (do l ol) (do (do a ol) o1) (do (do (do b ob) ol) o2)) (do (merge (do l ol) (do a ol) (do (do (do b ob) ol) o2)) o1)) = ()
-
-let inter_right_base_2op_comm3 (l a b :concrete_st) (o1 o2 ob ol:op_t)
-  : Lemma (requires Add? (snd (snd o2)) /\ Rem? (snd (snd o1)) /\
-                    Rem? (snd (snd ob)) /\ Add? (snd (snd ol)) /\
-                    eq (merge l (do a o1) (do (do b ob) o2)) (do (merge l a (do (do b ob) o2)) o1) /\ //from ind_right_2op
-                    eq (merge (do l ol) (do (do a ol) o1) (do (do b ol) o2)) (do (merge (do l ol) (do a ol) (do (do b ol) o2)) o1))
-          (ensures eq (merge (do l ol) (do (do a ol) o1) (do (do (do b ob) ol) o2)) (do (merge (do l ol) (do a ol) (do (do (do b ob) ol) o2)) o1)) = ()
-
-let inter_right_base_2op_comm4 (l a b :concrete_st) (o1 o2 ob ol:op_t)
-  : Lemma (requires Rem? (snd (snd o2)) /\ Add? (snd (snd o1)) /\
-                    Rem? (snd (snd ob)) /\ Add? (snd (snd ol)) /\
-                    eq (merge l (do a o1) (do (do b ob) o2)) (do (merge l a (do (do b ob) o2)) o1) /\ //from ind_right_2op
-                    eq (merge (do l ol) (do (do a ol) o1) (do (do b ol) o2)) (do (merge (do l ol) (do a ol) (do (do b ol) o2)) o1))
-          (ensures eq (merge (do l ol) (do (do a ol) o1) (do (do (do b ob) ol) o2)) (do (merge (do l ol) (do a ol) (do (do (do b ob) ol) o2)) o1)) = ()
-
-let inter_right_base_2op l a b o1 o2 ob ol =
-  if Fst_then_snd? (rc o2 o1) then inter_right_base_2op_fts l a b o1 o2 ob ol
-  else (if Add? (snd (snd o2)) && Add? (snd (snd o1)) then inter_right_base_2op_comm1 l a b o1 o2 ob ol
-        else if Rem? (snd (snd o2)) && Rem? (snd (snd o1)) then inter_right_base_2op_comm2 l a b o1 o2 ob ol
-        else if Add? (snd (snd o2)) && Rem? (snd (snd o1)) then inter_right_base_2op_comm3 l a b o1 o2 ob ol
-        else inter_right_base_2op_comm4 l a b o1 o2 ob ol)
+let inter_right_base_2op l a b o1 o2 ob ol = ()
 
 let inter_left_base_2op l a b o1 o2 ob ol = ()
 
-let inter_right_2op_fts (l a b:concrete_st) (o1 o2 ob ol o:op_t)
-  : Lemma (requires Fst_then_snd? (rc o2 o1) /\ Fst_then_snd? (rc ob ol) /\
-                    (~ (Either? (rc o ob)) \/ Fst_then_snd? (rc o ol)) /\
-                    eq (merge (do l ol) (do (do a ol) o1) (do (do (do b ob) ol) o2)) (do (merge (do l ol) (do a ol) (do (do (do b ob) ol) o2)) o1))
-          (ensures eq (merge (do l ol) (do (do a ol) o1) (do (do (do (do b o) ob) ol) o2)) (do (merge (do l ol) (do a ol) (do (do (do (do b o) ob) ol) o2)) o1)) = ()
+let inter_right_2op l a b o1 o2 ob ol o = ()
 
-let inter_right_2op_comm1 (l a b:concrete_st) (o1 o2 ob ol o:op_t)
-  : Lemma (requires Add? (snd (snd o2)) /\ Add? (snd (snd o1)) /\ get_rid o1 <> get_rid o2 /\
-                    Rem? (snd (snd ob)) /\ Add? (snd (snd ol)) /\ get_ele ob = get_ele ol /\
-                    (~ (Either? (rc o ob)) \/ Fst_then_snd? (rc o ol)) /\
-                    get_rid o <> get_rid ol /\
-                    eq (merge (do l ol) (do (do a ol) o1) (do (do (do b ob) ol) o2)) (do (merge (do l ol) (do a ol) (do (do (do b ob) ol) o2)) o1))
-          (ensures eq (merge (do l ol) (do (do a ol) o1) (do (do (do (do b o) ob) ol) o2)) (do (merge (do l ol) (do a ol) (do (do (do (do b o) ob) ol) o2)) o1)) = ()
+let inter_left_2op l a b o1 o2 ob ol o = ()
 
-let inter_right_2op_comm2 (l a b:concrete_st) (o1 o2 ob ol o:op_t)
-  : Lemma (requires Rem? (snd (snd o2)) /\ Rem? (snd (snd o1)) /\
-                    Rem? (snd (snd ob)) /\ Add? (snd (snd ol)) /\
-                    (~ (Either? (rc o ob)) \/ Fst_then_snd? (rc o ol)) /\
-                    get_rid o <> get_rid ol /\
-                    eq (merge (do l ol) (do (do a ol) o1) (do (do (do b ob) ol) o2)) (do (merge (do l ol) (do a ol) (do (do (do b ob) ol) o2)) o1))
-          (ensures eq (merge (do l ol) (do (do a ol) o1) (do (do (do (do b o) ob) ol) o2)) (do (merge (do l ol) (do a ol) (do (do (do (do b o) ob) ol) o2)) o1)) = ()
+let inter_lca_2op l a b o1 o2 ol = ()
 
-let inter_right_2op_comm3 (l a b:concrete_st) (o1 o2 ob ol o:op_t)
-  : Lemma (requires Add? (snd (snd o2)) /\ Rem? (snd (snd o1)) /\ get_ele o1 <> get_ele o2 /\
-                    Rem? (snd (snd ob)) /\ Add? (snd (snd ol)) /\ get_ele ob = get_ele ol /\
-                    (~ (Either? (rc o ob)) \/ Fst_then_snd? (rc o ol)) /\
-                    get_rid o <> get_rid ol /\
-                    eq (merge (do l ol) (do (do a ol) o1) (do (do (do b ob) ol) o2)) (do (merge (do l ol) (do a ol) (do (do (do b ob) ol) o2)) o1))
-          (ensures eq (merge (do l ol) (do (do a ol) o1) (do (do (do (do b o) ob) ol) o2)) (do (merge (do l ol) (do a ol) (do (do (do (do b o) ob) ol) o2)) o1)) = ()
+let ind_right_2op l a b o1 o2 o2' = ()
 
-let inter_right_2op_comm4 (l a b:concrete_st) (o1 o2 ob ol o:op_t)
-  : Lemma (requires Rem? (snd (snd o2)) /\ Add? (snd (snd o1)) /\ get_ele o1 <> get_ele o2 /\
-                    Rem? (snd (snd ob)) /\ Add? (snd (snd ol)) /\ get_ele ob = get_ele ol /\
-                    (~ (Either? (rc o ob)) \/ Fst_then_snd? (rc o ol)) /\
-                    get_rid o <> get_rid ol /\
-                    eq (merge (do l ol) (do (do a ol) o1) (do (do (do b ob) ol) o2)) (do (merge (do l ol) (do a ol) (do (do (do b ob) ol) o2)) o1))
-          (ensures eq (merge (do l ol) (do (do a ol) o1) (do (do (do (do b o) ob) ol) o2)) (do (merge (do l ol) (do a ol) (do (do (do (do b o) ob) ol) o2)) o1)) = ()
-
-let inter_right_2op l a b o1 o2 ob ol o =
-  if Fst_then_snd? (rc o2 o1) then inter_right_2op_fts l a b o1 o2 ob ol o
-  else (if Add? (snd (snd o2)) && Add? (snd (snd o1)) then inter_right_2op_comm1 l a b o1 o2 ob ol o
-        else if Rem? (snd (snd o2)) && Rem? (snd (snd o1)) then inter_right_2op_comm2 l a b o1 o2 ob ol o
-        else if Add? (snd (snd o2)) && Rem? (snd (snd o1)) then inter_right_2op_comm3 l a b o1 o2 ob ol o
-        else inter_right_2op_comm4 l a b o1 o2 ob ol o)
-
-let inter_left_2op (l a b:concrete_st) (o1 o2 ob ol o:op_t)
-  : Lemma (requires Rem? (snd (snd o2)) /\ Add? (snd (snd o1)) /\
-                    Rem? (snd (snd ob)) /\ Add? (snd (snd ol)) /\
-                    (~ (Either? (rc o ob)) \/ Fst_then_snd? (rc o ol)) /\
-                    get_rid o <> get_rid ol /\ //from app.fsti
-                    eq (merge (do l ol) (do (do (do a ob) ol) o1) (do (do b ol) o2)) (do (merge (do l ol) (do (do a ob) ol) (do (do b ol) o2)) o1))
-          (ensures eq (merge (do l ol) (do (do (do (do a o) ob) ol) o1) (do (do b ol) o2)) (do (merge (do l ol) (do (do (do a o) ob) ol) (do (do b ol) o2)) o1)) = ()
-
-let inter_lca_2op_fts (l a b:concrete_st) (o1 o2 ol:op_t)
-  : Lemma (requires Rem? (snd (snd o2)) /\ Add? (snd (snd o1)) /\
-                    Add? (snd (snd ol)) /\
-                    eq (merge (do l ol) (do (do a ol) o1) (do b ol)) (do (merge (do l ol) (do a ol) (do b ol)) o1) /\ //1op
-                    eq (merge l (do a o1) (do b o2)) (do (merge l a (do b o2)) o1))
-          (ensures eq (merge (do l ol) (do (do a ol) o1) (do (do b ol) o2)) (do (merge (do l ol) (do a ol) (do (do b ol) o2)) o1)) = ()
-
-let inter_lca_2op_comm1 (l a b:concrete_st) (o1 o2 ol:op_t)
-  : Lemma (requires Add? (snd (snd o2)) /\ Add? (snd (snd o1)) /\ get_rid o1 <> get_rid o2 /\
-                    Add? (snd (snd ol)) /\
-                    eq (merge (do l ol) (do (do a ol) o1) (do b ol)) (do (merge (do l ol) (do a ol) (do b ol)) o1) /\ //1op
-                    eq (merge l (do a o1) (do b o2)) (do (merge l a (do b o2)) o1))
-          (ensures eq (merge (do l ol) (do (do a ol) o1) (do (do b ol) o2)) (do (merge (do l ol) (do a ol) (do (do b ol) o2)) o1)) = ()
-
-let inter_lca_2op_comm2 (l a b:concrete_st) (o1 o2 ol:op_t)
-  : Lemma (requires Rem? (snd (snd o2)) /\ Rem? (snd (snd o1)) /\
-                    Add? (snd (snd ol)) /\
-                    eq (merge (do l ol) (do (do a ol) o1) (do b ol)) (do (merge (do l ol) (do a ol) (do b ol)) o1) /\ //1op
-                    eq (merge l (do a o1) (do b o2)) (do (merge l a (do b o2)) o1))
-          (ensures eq (merge (do l ol) (do (do a ol) o1) (do (do b ol) o2)) (do (merge (do l ol) (do a ol) (do (do b ol) o2)) o1)) = ()
-
-let inter_lca_2op_comm3 (l a b:concrete_st) (o1 o2 ol:op_t)
-  : Lemma (requires Add? (snd (snd o2)) /\ Rem? (snd (snd o1)) /\ get_ele o1 <> get_ele o2 /\
-                    Add? (snd (snd ol)) /\
-                    eq (merge (do l ol) (do (do a ol) o1) (do b ol)) (do (merge (do l ol) (do a ol) (do b ol)) o1) /\ //1op
-                    eq (merge l (do a o1) (do b o2)) (do (merge l a (do b o2)) o1))
-          (ensures eq (merge (do l ol) (do (do a ol) o1) (do (do b ol) o2)) (do (merge (do l ol) (do a ol) (do (do b ol) o2)) o1)) = ()
-
-let inter_lca_2op_comm4 (l a b:concrete_st) (o1 o2 ol:op_t)
-  : Lemma (requires Rem? (snd (snd o2)) /\ Add? (snd (snd o1)) /\ get_ele o1 <> get_ele o2 /\
-                    Add? (snd (snd ol)) /\
-                    eq (merge (do l ol) (do (do a ol) o1) (do b ol)) (do (merge (do l ol) (do a ol) (do b ol)) o1) /\ //1op
-                    eq (merge l (do a o1) (do b o2)) (do (merge l a (do b o2)) o1))
-          (ensures eq (merge (do l ol) (do (do a ol) o1) (do (do b ol) o2)) (do (merge (do l ol) (do a ol) (do (do b ol) o2)) o1)) = ()
-
-let inter_lca_2op l a b o1 o2 ol =
-  if Fst_then_snd? (rc o2 o1) then inter_lca_2op_fts l a b o1 o2 ol
-  else (if Add? (snd (snd o2)) && Add? (snd (snd o1)) then inter_lca_2op_comm1 l a b o1 o2 ol
-        else if Rem? (snd (snd o2)) && Rem? (snd (snd o1)) then inter_lca_2op_comm2 l a b o1 o2 ol
-        else if Add? (snd (snd o2)) && Rem? (snd (snd o1)) then inter_lca_2op_comm3 l a b o1 o2 ol
-        else inter_lca_2op_comm4 l a b o1 o2 ol)
-
-let ind_right_2op (l a b:concrete_st) (o1 o2 o2':op_t)
-  : Lemma (requires Rem? (snd (snd o2)) /\ Add? (snd (snd o1)) /\ get_ele o1 = get_ele o2 /\
-                    eq (merge l (do a o1) (do b o2)) (do (merge l a (do b o2)) o1))
-          (ensures eq (merge l (do a o1) (do (do b o2') o2)) (do (merge l a (do (do b o2') o2)) o1)) = ()
-
-let ind_left_2op_fts (l a b:concrete_st) (o1 o2 o1':op_t)
-  : Lemma (requires Rem? (snd (snd o2)) /\ Add? (snd (snd o1)) /\ get_ele o1 = get_ele o2 /\
-                    eq (merge l (do a o1) (do b o2)) (do (merge l a (do b o2)) o1))
-          (ensures eq (merge l (do (do a o1') o1) (do b o2)) (do (merge l (do a o1') (do b o2)) o1)) = ()
-
-let ind_left_2op_comm1 (l a b:concrete_st) (o1 o2 o1':op_t)
-  : Lemma (requires Add? (snd (snd o2)) /\ Add? (snd (snd o1)) /\
-                    eq (merge l (do a o1) (do b o2)) (do (merge l a (do b o2)) o1))
-          (ensures eq (merge l (do (do a o1') o1) (do b o2)) (do (merge l (do a o1') (do b o2)) o1)) = ()
-
-let ind_left_2op_comm2 (l a b:concrete_st) (o1 o2 o1':op_t)
-  : Lemma (requires Rem? (snd (snd o2)) /\ Rem? (snd (snd o1)) /\
-                    eq (merge l (do a o1) (do b o2)) (do (merge l a (do b o2)) o1))
-          (ensures eq (merge l (do (do a o1') o1) (do b o2)) (do (merge l (do a o1') (do b o2)) o1)) = ()
-
-let ind_left_2op_comm3 (l a b:concrete_st) (o1 o2 o1':op_t)
-  : Lemma (requires Add? (snd (snd o2)) /\ Rem? (snd (snd o1)) /\
-                    eq (merge l (do a o1) (do b o2)) (do (merge l a (do b o2)) o1))
-          (ensures eq (merge l (do (do a o1') o1) (do b o2)) (do (merge l (do a o1') (do b o2)) o1)) = ()
-
-let ind_left_2op_comm4 (l a b:concrete_st) (o1 o2 o1':op_t)
-  : Lemma (requires Rem? (snd (snd o2)) /\ Add? (snd (snd o1)) /\
-                    eq (merge l (do a o1) (do b o2)) (do (merge l a (do b o2)) o1))
-          (ensures eq (merge l (do (do a o1') o1) (do b o2)) (do (merge l (do a o1') (do b o2)) o1)) = ()
-
-let ind_left_2op l a b o1 o2 o1' =
-  if Fst_then_snd? (rc o2 o1) then ind_left_2op_fts l a b o1 o2 o1'
-  else (if Add? (snd (snd o2)) && Add? (snd (snd o1)) then ind_left_2op_comm1 l a b o1 o2 o1'
-        else if Rem? (snd (snd o2)) && Rem? (snd (snd o1)) then ind_left_2op_comm2 l a b o1 o2 o1'
-        else if Add? (snd (snd o2)) && Rem? (snd (snd o1)) then ind_left_2op_comm3 l a b o1 o2 o1'
-        else ind_left_2op_comm4 l a b o1 o2 o1')
+let ind_left_2op l a b o1 o2 o1' = ()
 
 let base_1op o1 = ()
 
 let ind_lca_1op l o1 ol = ()
 
-let inter_right_base_1op (l a b :concrete_st) (o1 ob ol:op_t)
-  : Lemma (requires Rem? (snd (snd ob)) /\ Add? (snd (snd ol)) /\
-                    (Fst_then_snd? (rc ob o1) ==> eq (merge l (do a o1) (do b ob)) (do (merge l a (do b ob)) o1)) /\ //from app.fsti
-                    eq (merge (do l ol) (do (do a ol) o1) (do b ol)) (do (merge (do l ol) (do a ol) (do b ol)) o1))
-          (ensures eq (merge (do l ol) (do (do a ol) o1) (do (do b ob) ol)) (do (merge (do l ol) (do a ol) (do (do b ob) ol)) o1)) = ()
+let inter_right_base_1op l a b o1 ob ol = ()
 
-let inter_left_base_1op (l a b:concrete_st) (o1 ob ol:op_t)
-  : Lemma (requires Rem? (snd (snd ob)) /\ Add? (snd (snd ol)) /\
-                    eq (merge (do l ol) (do (do a ol) o1) (do b ol)) (do (merge (do l ol) (do a ol) (do b ol)) o1))
-          (ensures eq (merge (do l ol) (do (do (do a ob) ol) o1) (do b ol)) (do (merge (do l ol) (do (do a ob) ol) (do b ol)) o1)) = ()
+let inter_left_base_1op l a b o1 ob ol = ()
 
-let inter_right_1op (l a b:concrete_st) (o1 ob ol o:op_t)
-  : Lemma (requires Rem? (snd (snd ob)) /\ Add? (snd (snd ol)) /\ get_ele ob = get_ele ol /\
-                    (~ (Either? (rc o ob)) \/ Fst_then_snd? (rc o ol)) /\
-                    get_rid o <> get_rid ol /\ //from app.fsti
-                    eq (merge (do l ol) (do (do a ol) o1) (do (do b ob) ol)) (do (merge (do l ol) (do a ol) (do (do b ob) ol)) o1))
-          (ensures eq (merge (do l ol) (do (do a ol) o1) (do (do (do b o) ob) ol)) (do (merge (do l ol) (do a ol) (do (do (do b o) ob) ol)) o1)) = ()
+let inter_right_1op l a b o1 ob ol o = ()
 
-let inter_left_1op (l a b:concrete_st) (o1 ob ol o:op_t)
-  : Lemma (requires Rem? (snd (snd ob)) /\ Add? (snd (snd ol)) /\ get_ele ob = get_ele ol /\
-                    (~ (Either? (rc o ob)) \/ Fst_then_snd? (rc o ol)) /\
-                    get_rid o <> get_rid ol /\ //from app.fsti
-                    eq (merge (do l ol) (do (do (do a ob) ol) o1) (do b ol)) (do (merge (do l ol) (do (do a ob) ol) (do b ol)) o1))
-          (ensures eq (merge (do l ol) (do (do (do (do a o) ob) ol) o1) (do b ol)) (do (merge (do l ol) (do (do (do a o) ob) ol) (do b ol)) o1)) = ()
+let inter_left_1op l a b o1 ob ol o = ()
 
-let inter_lca_1op (l a b:concrete_st) (o1 ol oi:op_t)
-  : Lemma (requires Add? (snd (snd ol)) /\ Add? (snd (snd oi)) /\
-                    eq (merge (do l oi) (do (do a oi) o1) (do b oi)) (do (merge (do l oi) (do a oi) (do b oi)) o1) /\
-                    eq (merge (do l ol) (do (do a ol) o1) (do b ol)) (do (merge (do l ol) (do a ol) (do b ol)) o1))
-          (ensures eq (merge (do (do l oi) ol) (do (do (do a oi) ol) o1) (do (do b oi) ol))
-                      (do (merge (do (do l oi) ol) (do (do a oi) ol) (do (do b oi) ol)) o1)) = ()
+let inter_lca_1op l a b o1 ol oi = ()
 
-let ind_left_1op (l a b:concrete_st) (o1 o1' ol:op_t)
-  : Lemma (requires eq (merge (do l ol) (do a o1) (do b ol)) (do (merge (do l ol) a (do b ol)) o1))
-          (ensures eq (merge (do l ol) (do (do a o1') o1) (do b ol)) (do (merge (do l ol) (do a o1') (do b ol)) o1)) = ()
+let ind_left_1op l a b o1 o1' ol = ()
 
-let ind_right_1op (l a b:concrete_st) (o2 o2' ol:op_t)
-  : Lemma (requires eq (merge (do l ol) (do a ol) (do b o2)) (do (merge (do l ol) (do a ol) b) o2))
-          (ensures eq (merge (do l ol) (do a ol) (do (do b o2') o2)) (do (merge (do l ol) (do a ol) (do b o2')) o2)) = ()
+let ind_right_1op l a b o2 o2' ol = ()
 
 let lem_0op l a b ol = ()
+
+#pop-options
